Update tlb invalidation definitions

ArchSemArm/VMPromising.v
@@ -989,11 +989,159 @@ Module TLB.
     tlb1 ← va_fill tlb0 ts init mem time 1%fin va ttbr;
     tlb2 ← va_fill tlb1 ts init mem time 2%fin va ttbr;
     va_fill tlb2 ts init mem time 3%fin va ttbr.
+
+  (** ** TLB invalidation *)
+
+  Definition affects_va (asid : bv 16) (va : bv 36) (last : bool)
+                        (ctxt : Ctxt.t)
+                        (te : Entry.t (Ctxt.lvl ctxt)) : Prop :=
+    let '(te_lvl, te_va, te_asid, te_val) :=
+          (Ctxt.lvl ctxt, Ctxt.va ctxt, Ctxt.asid ctxt, Entry.pte te) in
+    (match_prefix_at te_lvl te_va va)
+    ∧ (match te_asid with
+        | Some te_asid => asid = te_asid
+        | None => True
+        end)
+    ∧ (if last then is_final te_lvl te_val else False).
+  Instance Decision_affects_va (asid : bv 16) (va : bv 36) (last : bool)
+                               (ctxt : Ctxt.t)
+                               (te : Entry.t (Ctxt.lvl ctxt)) :
+    Decision (affects_va asid va last ctxt te).
+  Proof. unfold_decide. Defined.
+
+  Definition affects_asid (asid : bv 16)
+                          (ctxt : Ctxt.t)
+                          (te : Entry.t (Ctxt.lvl ctxt)) : Prop :=
+    match (Ctxt.asid ctxt) with
+    | Some te_asid => te_asid = asid
+    | None => False
+    end.
+  Instance Decision_affects_asid (asid : bv 16)
+                                 (ctxt : Ctxt.t)
+                                 (te : Entry.t (Ctxt.lvl ctxt)) :
+    Decision (affects_asid asid ctxt te).
+  Proof. unfold_decide. Defined.
+
+  Definition affects_vaa (va : bv 36) (last : bool)
+                         (ctxt : Ctxt.t)
+                         (te : Entry.t (Ctxt.lvl ctxt)) : Prop :=
+    let '(te_lvl, te_va, te_val) :=
+          (Ctxt.lvl ctxt, Ctxt.va ctxt, Entry.pte te) in
+    (match_prefix_at te_lvl te_va va)
+    ∧ (if last then is_final te_lvl te_val else False).
+  Instance Decision_affects_vaa (va : bv 36) (last : bool)
+                                (ctxt : Ctxt.t)
+                                (te : Entry.t (Ctxt.lvl ctxt)) :
+    Decision (affects_vaa va last ctxt te).
+  Proof. unfold_decide. Defined.
+
+  Definition affects (tlbi : TLBI.t) (ctxt : Ctxt.t)
+                     (te : Entry.t (Ctxt.lvl ctxt)) : Prop :=
+    match tlbi with
+    | TLBI.All tid => True
+    | TLBI.Va tid asid va last => affects_va asid va last ctxt te
+    | TLBI.Asid tid asid => affects_asid asid ctxt te
+    | TLBI.Vaa tid va last => affects_vaa va last ctxt te
+    end.
+  Instance Decision_affects (tlbi : TLBI.t) (ctxt : Ctxt.t)
+                     (te : Entry.t (Ctxt.lvl ctxt)) :
+    Decision (affects tlbi ctxt te).
+  Proof. unfold_decide. Defined.
+
+  Definition tlbi_apply_lvl (tlb : t) (ts : TState.t)
+                  (init : Memory.initial) (mem : Memory.t)
+                  (time : nat)
+                  (tlbi : TLBI.t)
+                  (lvl : Level)
+                  (va : bv 64)
+                  (asid : option (bv 16)) : t :=
+    let ndctxt := NDCtxt.make (level_prefix va lvl) asid in
+    let ctxt := existT lvl ndctxt in
+    VATLB.get ctxt tlb.(vatlb)
+    |> filter (λ te, ¬(affects tlbi ctxt te))
+    |> λ tes,
+        TLB.make $ hset (Ctxt.lvl ctxt) {[(Ctxt.nd ctxt) := tes]} tlb.(vatlb).
+
+  Definition tlbi_apply (tlb : t) (ts : TState.t)
+                  (init : Memory.initial) (mem : Memory.t)
+                  (time : nat)
+                  (tlbi : TLBI.t)
+                  (va : bv 64)
+                  (asid : option (bv 16)) : t :=
+    let tlb0 := tlbi_apply_lvl tlb ts init mem time tlbi root_lvl va asid in
+    let tlb1 := tlbi_apply_lvl tlb0 ts init mem time tlbi 1%fin va asid in
+    let tlb2 := tlbi_apply_lvl tlb1 ts init mem time tlbi 2%fin va asid in
+    tlbi_apply_lvl tlb2 ts init mem time tlbi 3%fin va asid.
+
+  (** Get the TLB state at a certain timestamp *)
+  Fixpoint at_timestamp (ts : TState.t) (mem_init : Memory.initial) (mem : Memory.t)
+                       (time : nat)
+                       (va : bv 64)
+                       (asid : option (bv 16))
+                       (ttbr : reg)
+                      {struct time} : result string t :=
+    match time with
+    | O => update init ts mem_init mem 0 va ttbr
+    | S ptime =>
+      tlb ← at_timestamp ts mem_init mem ptime va asid ttbr;
+      match mem !! time with
+      | Some ev =>
+        match Ev.get_tlbi ev with
+        | Some tlbi => mret $ tlbi_apply tlb ts mem_init mem time tlbi va asid
+        | None => update tlb ts mem_init mem time va ttbr
+        end
+      | None => mret init
+      end
+    end.
+
+  Definition is_te_invalidated_by_tlbi (tlb : t)
+                (tlbi : TLBI.t)
+                (tid : nat)
+                (ctxt : Ctxt.t)
+                (te : Entry.t (Ctxt.lvl ctxt)) : Prop :=
+      TLBI.tid tlbi <> tid ∧ te ∉ VATLB.get ctxt tlb.(vatlb).
+  Instance Decision_is_te_invalidated_by_tlbi (tlb : t) (tlbi : TLBI.t) (tid : nat)
+                (ctxt : Ctxt.t) (te : Entry.t (Ctxt.lvl ctxt)) :
+    Decision (is_te_invalidated_by_tlbi tlb tlbi tid ctxt te).
+  Proof. unfold_decide. Defined.
+
+  Fixpoint invalidation_time_from_evs (ts : TState.t) (init : Memory.initial)
+                                      (mem : Memory.t)
+                                      (tid : nat)
+                                      (ctxt : Ctxt.t)
+                                      (te : Entry.t (Ctxt.lvl ctxt))
+                                      (ttbr : reg)
+                                      (evs : list (Ev.t * nat)) : result string nat :=
+    match evs with
+    | nil => mret 0
+    | (ev, t) :: tl =>
+      match ev with
+      | Ev.Tlbi tlbi =>
+        let va := Ctxt.va ctxt in
+        let asid := Ctxt.asid ctxt in
+        tlb ← at_timestamp ts init mem t (prefix_to_va va) asid ttbr;
+        if decide (is_te_invalidated_by_tlbi tlb tlbi tid ctxt te) then
+          mret t
+        else
+          invalidation_time_from_evs ts init mem tid ctxt te ttbr tl
+      | _ => invalidation_time_from_evs ts init mem tid ctxt te ttbr tl
+      end
+    end.
+
+  (** Calculate the earliest future time at which a translation entry is effectively invalidated
+      in the TLB due to an TLBI event *)
+  Definition invalidation_time (ts : TState.t) (init : Memory.initial) (mem : Memory.t)
+                               (tid : nat) (time : nat)
+                               (ctxt : Ctxt.t)
+                               (te : Entry.t (Ctxt.lvl ctxt))
+                               (ttbr : reg) : result string nat :=
+    let evs := PromMemory.cut_after_with_timestamps time mem in
+    invalidation_time_from_evs ts init mem tid ctxt te ttbr evs.
 End TLB.
 
 Module VATLB := TLB.VATLB.
 
-(*** Instruction semantics ***)
+(** * Instruction semantics ***)
 
 (** Intra instruction state for propagating views inside an instruction *)
 Module IIS.
